theories/fae.v
@@ -1,0 +1,50 @@
+From fae_gtlc_mu.stlc_mu Require Export contexts.
+From fae_gtlc_mu.cast_calculus Require Export contexts.
+From fae_gtlc_mu.embedding Require Export expressions types.
+From fae_gtlc_mu.backtranslation Require Export contexts.
+From fae_gtlc_mu.refinements.static_gradual Require Export soundness.
+From fae_gtlc_mu.refinements.static_gradual Require Export rel_ref_specs.
+
+Notation "Γ ⊨ e '=ctx-grad=' e' : τ" :=
+  (cast_calculus.contexts.ctx_equiv Γ e e' τ) (at level 74, e, e', τ at next level).
+
+Notation "Γ ⊨ e '=ctx-stat=' e' : τ" :=
+  (stlc_mu.contexts.ctx_equiv Γ e e' τ) (at level 74, e, e', τ at next level).
+
+Lemma static_ctx_refines_gradual (Γ : list stlc_mu.typing.type) (e : stlc_mu.lang.expr) (τ : stlc_mu.typing.type) (de : Γ ⊢ₛ e : τ) :
+  ∀ (Cₜ : cast_calculus.contexts.ctx), cast_calculus.contexts.typed_ctx Cₜ (map embed_type Γ) (embed_type τ) [] TUnit →
+     Halts_stat (stlc_mu.contexts.fill_ctx (backtranslate_ctx Cₜ) e) →
+     Halts_grad (fill_ctx Cₜ [[e]]).
+Proof.
+  intros Cₜ dCₜ Hs.
+  apply (@soundness actualΣ _ _ (stlc_mu.contexts.fill_ctx (backtranslate_ctx Cₜ) e) _ TUnit).
+  intros.
+  eapply back_ctx_relates. admit. admit. apply dCₜ.
+  apply embedding_relates; done.
+  done.
+Admitted.
+
+Lemma gradual_ctx_refines_static (Γ : list stlc_mu.typing.type) (e : stlc_mu.lang.expr) (τ : stlc_mu.typing.type) :
+  ∀ (K : cast_calculus.contexts.ctx), cast_calculus.contexts.typed_ctx K (map embed_type Γ) (embed_type τ) [] TUnit →
+     Halts_grad (fill_ctx K [[e]]) →
+     Halts_stat (stlc_mu.contexts.fill_ctx (backtranslate_ctx K) e).
+Proof.
+Admitted.
+
+
+Theorem ctx_eq_preservation Γ e1 e2 τ (Hctx : Γ ⊨ e1 =ctx-stat= e2 : τ) :
+  map embed_type Γ ⊨ [[e1]] =ctx-grad= [[e2]] : embed_type τ.
+Proof.
+  split; try split. admit. admit.
+  intros Cₜ dCₜ. split.
+  - intro Hg1.
+    apply (static_ctx_refines_gradual Γ e2 τ (ltac:(apply Hctx)) Cₜ dCₜ).
+    apply Hctx. admit.
+    apply (gradual_ctx_refines_static Γ e1 τ Cₜ dCₜ).
+    apply Hg1.
+  - intro Hg2.
+    apply (static_ctx_refines_gradual Γ e1 τ (ltac:(apply Hctx)) Cₜ dCₜ).
+    apply Hctx. admit.
+    apply (gradual_ctx_refines_static Γ e2 τ Cₜ dCₜ).
+    apply Hg2.
+Admitted.
